\chapter{TENSOR PRODUCT}

\section{TENSOR PRODUCT OF MODULES}

\begin{definition}[bilinear map, multilinear map]
	Let $M, N, L$ be $A$-modules. A map $b: M \times N \to L$ is $A$-bilinear if it is $A$-linear in each component, that is
	\begin{align*}
		b(m_1 + m_2, n) &= b(m_1, n) + b(m_2, n) \\
		b(m, n_1 + n_2) &= b(m, n_1) + b(m, n_2) \\
		a b(m, b) &= b(am, n) = b(m, an)
	\end{align*}
	
	for all $a \in A$, $m_1, m_2 \in M$, and $n_1, n_2 \in N$. The set of all $A$-bilinear maps $M \times N \to L$ is denoted by
	$$
		\Bil_A(M \times N, L)
	$$
	
	and it carries a $A$-module structure induced from $L$, that is
	\begin{align*}
		(f + g)(m, n) &= f(m, n) + g(m, n) \\
		(a f)(m, n) &= a f(m, n)
	\end{align*}
	
	Similar definition for $A$-multilinear maps
\end{definition}

\begin{theorem}[tensor product]
	Let $M, N$ be $A$-modules, there exists an $A$-module denoted by $M \otimes_A N$ together with a bilinear map $b_{univ}: M \times N \to M \otimes N$ so that for every $A$-module $L$ the map below is an $A$-module isomorphism
	\begin{align*}
		\Hom_A(M \otimes_A N, L) &\xrightarrow{\sim} \Bil_A(M \times N, L) \\
		f &\mapsto f b_{univ}
	\end{align*}
\end{theorem}

\begin{proof}[Construction]
	Let $F$ be the free $A$-module generated by $M \times N$. Let $R \subseteq F$ be the submodule generated by the elements
	\begin{align*}
		&(m + m_1, n) - (m, n) - (m_1, n) \\
		&(m, n + n_1) - (m, n) - (m, n_1) \\
		&a (m, n) - (am, n) \\
		&a(m, n) - (m, an)
	\end{align*}
	
	for all $a \in A$, $m, m_1 \in M$, and $n, n_1 \in N$. Set $M \otimes N = F / R$. Let the equivalence class of $(m, n)$ denoted by $m \otimes n$. Define
	\begin{align*}
		b_{univ}: M \times N &\to M \otimes N \\
		(m, n) &\mapsto m \otimes n
	\end{align*}
\end{proof}

\begin{proof}
	It is clear that the composition $f b_{univ}$ is bilinear. Conversely, consider the bilinear map $b: M \times N \to L$, define
	\begin{align*}
		\tilde{b}: F &\to L \\
		\sum_{i} a_i (m_i, n_i) &\mapsto \sum_{i} a_i b(m_i, n_i)
	\end{align*}
	
	As $R \subseteq \tilde{b}$, by property of kernel, $\tilde{b}$ factors through $F / R = M \otimes N$ by a unique map $\beta: M \otimes N \to L$
	\begin{center}
		\begin{tikzcd}
			M \times N \arrow[r, hook] \arrow[d, "b"'] & F \arrow[r, two heads] \arrow[ld, "\tilde{b}"'] & F / R = M \otimes N \arrow[lld, "\beta", dashed] \\
			L                                          &                                                 &                                                   
		\end{tikzcd}
	\end{center}
	
	The construction makes a pair of isomorphisms $\Hom(M \otimes N, L) \to \Bil(M \times N, L)$ and $\Bil(M \times N, L) \to \Hom(M \otimes N, L)$.
\end{proof}

\begin{proposition}
	Some properties of tensor product induced from the universal property
	\begin{align*}
		M \otimes A &= A \otimes M = A \\
		M \otimes N &\cong N \otimes M &\text{(since $\Bil(M \times N, L) \cong \Bil(N \times M, L)$)} \\
		(M_1 \oplus M_2) \otimes N &\cong (M_1 \otimes N) \oplus (M_2 \otimes N) \\
		(M \otimes N) \otimes L &\cong M \otimes (N \otimes L)
	\end{align*}
\end{proposition}

\begin{remark}[associativity of tensor product for modules of non-commutative rings]
	Let $A$ and $B$ be any ring (possibly non-commutative), $M$ be a right $A$-module, $N$ be a left $B$-module, and $L$ be a $(A, B)$-bimodule. Then, $M \otimes_A L$ and $L \otimes_B N$ are $(A, B)$-bimodules and 
	$$
		(M \otimes_A L) \otimes_B N \cong M \otimes_A (L \otimes_B N)
	$$
\end{remark}

\begin{remark}[tensor product as a functor]
	Let $f_1: M_1 \to N_1$ and $g: M_2 \to N_2$ be $A$-module morphisms, there is an induced $A$-module morphism defined by
	\begin{align*}
		f \otimes g: M_1 \otimes M_2 &\to N_1 \otimes N_1 \\
							m_1 \otimes m_2 &\mapsto f(m_1) \otimes f(m_1)
 	\end{align*}
	
	Then $(- \otimes L)$ can be defined as a functor from $A$-module into $A$-module. For any $A$-module morphism $f: M \to N$, the induced morphism is defined by $f \otimes 1_L: M \otimes L \to N \otimes L$
\end{remark}

\begin{remark}[extension of scalars]
	Let $\phi: A \to B$ is a ring map, $B$ is naturally an $A$-algebra
	\begin{align*}
				A \times B &\to B \\
					(a, b) &\mapsto a b = \phi(a) b
	\end{align*}

	If $M$ is an $A$-module and, then $M \otimes_A B$ carries a $B$-module structure with scalar multiplication in $B$-module defined by
	\begin{align*}
		B \times (M \otimes_A B) &\to M \otimes_A B \\
		(b, m_i \otimes b_i) &\mapsto m_i \otimes b b_i
	\end{align*}
	
	The scalar multiplication is compatible with $A$-module, that is,
	\begin{align*}
		\phi(a) (m \otimes b) 
		&= m \otimes \phi(a) b \\
		&= m \otimes ab \\
		&= am \otimes b \\
		&= a(m \otimes b)
	\end{align*}
	
	Any ring map $\phi: A \to B$ induces a functor from $A$-module into $B$-module defined by $(- \otimes_A B)$
\end{remark}

\begin{proof}
	\note{TODO}
\end{proof}

\begin{proposition}[localizing modules is tensor product]
	Let $S$ be a multiplicatively closed subset of a ring $A$ and $M$ be an $A$-module, then there exists a canonical isomorphism of $S^{-1} A$-module
	$$
		(S^{-1} A) \otimes_A M \xrightarrow{\sim} S^{-1} M
	$$
\end{proposition}

\begin{proof}
	Define the map
	\begin{align*}
		(S^{-1} A) \times M &\to S^{-1} M \\
		\tuple*{\frac{a}{s}, m} &\mapsto \frac{am}{s}
	\end{align*}
	
	is $A$-bilinear that induces a unique $A$-module morphism
	\begin{align*}
		f: (S^{-1} A) \otimes M &\to S^{-1} M \\
		\frac{a}{s} \otimes m &\mapsto \frac{am}{s}
	\end{align*}
	
	this map is surjective since every $\frac{m}{s} \in S^{-1} M$ is mapped from $\frac{1}{s} \otimes m \in S^{-1} A \otimes M$. We will show that it is injective. Let $\sum_{i} \frac{a_i}{s_i} \otimes m_i \in S^{-1}A \otimes M$, let $s = \prod_{i} s_i$ and $t_i = \prod_{j \neq i} s_j$, then
	\begin{align*}
		\sum_{i} \frac{a_i}{s_i} \otimes m_i
		&= \sum_{i} \frac{t_i a_i}{s} \otimes m_i \\
		&= \sum_{i} \frac{1}{s} \otimes t_i a_i m_i \\
		&= \frac{1}{s} \otimes \sum_{i} t_i a_i m_i
	\end{align*}
	
	That is, every element of $S^{-1} A \otimes M$ is of the form $\frac{1}{s} \otimes m$ for some $s \in S$ and $m \in M$. Now, if $\frac{1}{s} \otimes m \in \ker f$, then $\frac{m}{s} = 0$ in $S^{-1} M$, then there exists $t \in S$ such that $tm = 0$. So
	$$
		\frac{1}{s} \otimes m = \frac{1}{ts} \otimes tm = 0
	$$
	
	Hence, $\ker f = 0$
\end{proof}

\begin{proposition}[tensor-hom adjunction]
	Let $M, N, L$ be $A$-modules, then
	$$
		\Hom(M \otimes N, L) \cong \Hom(M, \Hom(N, L))
	$$
\end{proposition}

\begin{proof}
	$
		\Hom(M \otimes N, L) \cong  \Bil(M \times N, L) \cong \Hom(M, \Hom(N, L))
	$
\end{proof}

\section{EXACTNESS OF TENSOR PRODUCT}

\begin{definition}[exact functor]
	For any exact sequence $0 \rightarrow M \rightarrow N \rightarrow L \rightarrow 0$
	
	Let $F$ be a covariant functor from $A$-module into $A$-module
	
	\begin{enumerate}
		\item $F$ is left exact if $0 \rightarrow F(M) \rightarrow F(N) \rightarrow F(L)$
		\item $F$ is right exact if $F(M) \rightarrow F(N) \rightarrow F(L) \rightarrow 0$
	\end{enumerate}
	
	Let $G$ be a contravariant functor from $A$-module into $A$-module
	
	\begin{enumerate}
		\item $G$ is left exact if $0 \to F(L) \to F(N) \to F(M)$
		\item $G$ is right exact if $F(L) \to F(N) \to F(M) \to 0$
	\end{enumerate}
	
	A functor is called exact if it is both left exact and right exact. 
	
	\note{note, one can prove that we don't require the original sequence $0 \rightarrow M \rightarrow N \rightarrow L \to 0$ to be complete}
\end{definition}

\begin{lemma}[$\Hom$ functors are left exact]
	For any $A$-module $P$, the covariant functor $\Hom(P, -)$ and the contravariant functor $\Hom(-, P)$ are \textbf{left exact}. That is, if the first row is exact then the following two rows are exact 
	
	\begin{center}
		\begin{tikzcd}
			0 \arrow[r, dashed] & M \arrow[r, "i"]                    & N \arrow[r, "p"]              & L \arrow[r, dashed] & 0 \\
			0 \arrow[r]         & {\Hom(P, M)} \arrow[r, "i_1", hook] & {\Hom(P, N)} \arrow[r, "p_1"] & {\Hom(P, L)}        &   \\
			0 \arrow[r]         & {\Hom(L, P)} \arrow[r, "p_2", hook] & {\Hom(N, P)} \arrow[r, "i_2"] & {\Hom(M, P)}        &  
		\end{tikzcd}
	\end{center}

	Moreover, the statement is if and only if. That is, if one of $\Hom$ sequences is exact for every $A$-module $P$, then the original sequence is exact
\end{lemma}

\begin{proof} \note{Below is a sketch proof for the ($\implies$) direction, the ($\impliedby$) direction can be constructed}
	
	($i$ is mono $\implies$ $i_1$ is mono) Let $a$ and $b$ be two maps in $\Hom(P, M)$, then $i_1(a) = ia, i_1(b) = ib$, since $i$ is mono, $ia = ib \implies a = b$, that is $i_1$ is mono
	
	\begin{center}
		\begin{tikzcd}
			M \arrow[r, "i", hook]                                                                                           & N \\
			P \arrow[u, "a"'] \arrow[ru, "ia", dashed] \arrow[u, "b", bend left] \arrow[ru, "ib"', dashed, bend right] &  
		\end{tikzcd}
	\end{center}
	
	($\im i \subseteq \ker p \implies \im i_1 \subseteq \ker p_1$) Let $a \in \Hom(P, M)$, then $p_1 i_1 (a) = pib$. As $pi = 0$, then $p_1 i_1 = 0$, that is $\im i_1 \subseteq \ker p_1$
	\begin{center}
		\begin{tikzcd}
			M \arrow[r, "i"]                                                 & N \arrow[r, "p"] & L \\
			P \arrow[u, "a"'] \arrow[ru, "ia", dashed] \arrow[rru, "pib"', dashed] &                  &  
		\end{tikzcd}
	\end{center}
	
	($i$ is mono and $\im i = \ker p \implies \im i_1 \supseteq \ker p_1$) Let $a \in \ker p_1$, that is $p_1(a) = pa = 0$. Since $i: M \to N$ is the kernel of $p: N \to L$, then $a$ factors uniquely through $i$ by a map $b: M \to P$. Hence, $a = i_1(b)$, that is $a \in \im i_1$
	\begin{center}
		\begin{tikzcd}
			M \arrow[r, "i", hook] & N \arrow[r, "p"]                                                  & L \\
			& P \arrow[ru, "0"', dashed] \arrow[u, "a"] \arrow[lu, "b", dashed] &  
		\end{tikzcd}
	\end{center}
	
	($p$ is epi $\implies$ $p_2$ is mono) Let $a$ and $b$ be two maps in $\Hom(L, P)$, then $p_2(a) = ap, p_2(b) = bp$, since $p$ is epi, $ap = bp \implies a = b$, that is $p_2$ is mono.
	\begin{center}
		\begin{tikzcd}
			& P                                            \\
			N \arrow[r, "p"', two heads] \arrow[ru, "ap"', dashed] \arrow[ru, "bp", dashed, bend left] & L \arrow[u, "a"] \arrow[u, "b"', bend right]
		\end{tikzcd}
	\end{center}
	
	($\im i \subseteq \ker p \implies \im p_2 \subseteq \ker i_2$) Let $a \in \Hom(L, P)$, then $i_2 p_2(a) = api$. As $pi = 0$, then $i_2 p_2 = 0$, that is $\im p_2 \subseteq \ker i_2$
	\begin{center}
		\begin{tikzcd}
			&                                                        & P                \\
			M \arrow[r, "i"'] \arrow[rru, "api", dashed] & N \arrow[ru, "ap"', dashed] \arrow[r, "p"', two heads] & L \arrow[u, "a"]
		\end{tikzcd}
	\end{center}
	
	($p$ is epi and $\im i = \ker p \implies \im p_2 \subseteq \ker i_2$) Let $a \in \ker i_2$, that is $i_2(a) = ai = 0$. Since $p: N \to L$ is the cokernel of $i: M \to N$, then $a$ factors uniquely through $p$ by a map $b: L \to P$. Hence, $a = p_2(b)$, that is $a \in \im p_2$
	\begin{center}
		\begin{tikzcd}
			& P                                           &                            \\
			M \arrow[r, "i"'] \arrow[ru, "0", dashed] & N \arrow[r, "p"', two heads] \arrow[u, "a"] & L \arrow[lu, "b"', dashed]
		\end{tikzcd}
	\end{center}
\end{proof}

\begin{proposition}[adjunction induces exact functors]
	Let $(F, G)$ be an adjunction of $A$-modules, that is, for any $A$-modules $M, N$, then 
	$$
		\Hom(F(M), N) \cong \Hom(M, G(N))
	$$

	Then, $F$ is right exact and $G$ is left exact
\end{proposition}

\begin{proof} For any $A$-module $P$
	
	($F$ is right exact) the following rows are exact
	\begin{center}
		\begin{tikzcd}
			& M \arrow[r]                                  & N \arrow[r]                                  & L \arrow[r]                        & 0 \\
			0 \arrow[r] & {\Hom(L, G(P))} \arrow[r] \arrow[d, "\sim"'] & {\Hom(N, G(P))} \arrow[r] \arrow[d, "\sim"'] & {\Hom(M, G(P))} \arrow[d, "\sim"'] &   \\
			0 \arrow[r] & {\Hom(F(L), P)} \arrow[r]                    & {\Hom(F(N), P)} \arrow[r]                    & {\Hom(F(M), P)}                    &   \\
			& F(M) \arrow[r]                               & F(N) \arrow[r]                               & F(L) \arrow[r]                     & 0
		\end{tikzcd}
	\end{center}
	
	($G$ is left exact) the following rows are are exact
	\begin{center}
		\begin{tikzcd}
			0 \arrow[r] & M \arrow[r]                                   & N \arrow[r]                                   & L                                   \\
			0 \arrow[r] & {\Hom(F(P), M)} \arrow[r] \arrow[d, "\sim"'] & {\Hom(F(P), N)} \arrow[r] \arrow[d, "\sim"'] & {\Hom(F(P), L)} \arrow[d, "\sim"'] \\
			0 \arrow[r] & {\Hom(P, G(M))} \arrow[r]                     & {\Hom(P, G(N))} \arrow[r]                     & {\Hom(P, G(L))}                     \\
			0 \arrow[r] & G(M) \arrow[r]                                & G(N) \arrow[r]                                & G(L)                               
		\end{tikzcd}
	\end{center}
\end{proof}

\begin{corollary}[tensor product is right exact]
	Tensor-hom adjunction $\Hom(M \otimes N, L) \cong \Hom(M, \Hom(N, L))$ where $F = (- \otimes N)$ and $G = \Hom(-, L)$. Then, $(- \otimes N)$ a right exact covariant functor. That is, for any $A$-module $P$, the following rows are exact
	\begin{center}
		\begin{tikzcd}
			M \arrow[r]           & N \arrow[r]           & L \arrow[r]           & 0 \\
			M \otimes P \arrow[r] & N \otimes P \arrow[r] & L \otimes P \arrow[r] & 0
		\end{tikzcd}
	\end{center}
\end{corollary}

\begin{definition}[flat module]
	An $A$-module $L$ is flat if the functor $(- \otimes L)$ is exact. Equivalently, for any injective map $M \hookrightarrow N$, the induced map $M \otimes L \hookrightarrow N \otimes L$ is also injective.
\end{definition}

\begin{proposition}
	Let $S$ be a multiplicatively closed subset of a ring $A$, then $S^{-1} A$ is flat.
\end{proposition}

\begin{proof}
	Since $(S^{-1} -)$ is an exact functor from $A$-module into $A$-module and $(S^{-1} -) = (S^{-1} A \otimes -)$. Then $S^{-1} A$ is flat.
\end{proof}

\begin{proposition}[flatness is a local property]
	Let $M$ be any $A$-module, the following are equivalent
	\begin{enumerate}
		\item $M$ is flat
		\item $M_\mf{p}$ is flat over $A_\mf{p}$ for every prime ideal $\mf{p}$ of $A$
		\item $M_\mf{m}$ is flat over $A_\mf{m}$ for every maximal ideal $\mf{m}$ of $A$
	\end{enumerate}
\end{proposition}

\begin{lemma}[useful calculation technique]
	Let $\phi: A \to B$ be a ring map, $I$ be an ideal of $B$ and $M$ be an $A$-module, then by right exactness of tensor product, the sequences below are exact
	\begin{center}
		\begin{tikzcd}
			0 \arrow[r] & I \arrow[r, "i", hook]                 & B \arrow[r, "p", two heads]        & B / I \arrow[r]           & 0 \\
			& I \otimes_A M \arrow[r, "i \otimes 1"] & B \otimes_A M \arrow[r, two heads] & B/I \otimes_A M \arrow[r] & 0
		\end{tikzcd}
	\end{center}
	
	Then, $B/I \otimes_A M = \coker (i \otimes 1)$. In particular, when $B = A$, $\phi = 1_A$ and $I$ is an ideal in $A$, then
	$$
		A / I \otimes_A M \cong M / IM
	$$
	
	when $B = A$, $I$ is an ideal of $A$ and $M = A/J$, then
	$$
		A / I \otimes_A A/J \cong A / (I + J)
	$$
\end{lemma}


\begin{longproof}
	($A / I \otimes_A M \cong M / IM$)

	\begin{center}
		\begin{tikzcd}
			I \otimes_A M \arrow[r, "i \otimes 1"] & A \otimes_A M \arrow[r, "\sim"]               & M  \\
			a \otimes m \arrow[r, maps to]         & a \otimes m \arrow[r, maps to] & am
		\end{tikzcd}
	\end{center}
	
	Every element $a \otimes m \in I \otimes_A M$ is mapped into the element $am \in M$, hence the image of $(i \otimes 1)$ in $M$ is $IM$. Hence, $\coker(i \otimes 1) \cong M / IM$
	
	($A / I \otimes_A A/J \cong A / (I + J)$)
	
	\begin{center}
		\begin{tikzcd}
			I \otimes_A A/J \arrow[r, "i \otimes 1"] & A \otimes_A A/J \arrow[r, "\sim"]               & A/J  \\
			a \otimes \bar{b} \arrow[r, maps to]         & a \otimes \bar{b} \arrow[r, maps to] & \overline{ab}
		\end{tikzcd}
	\end{center}
	
	Every element $a \otimes \bar{b} \in I \otimes_A A/J$ is mapped into the element $\overline{ab} \in A / J$ for $a \in I$ and $b \in A$. Hence, $\im (i \otimes 1)$ in $A/J$ is $\set{i + J: i \in I} = I / J = (I + J) / J$, then
	$$
		\coker (i \otimes 1) = \frac{A / J}{(I + J) / J} = \frac{A}{I + J}
	$$
\end{longproof}

\section{TENSOR PRODUCT OF ALGEBRAS}

\begin{theorem}[tensor product of algebras]
	Let $B$ and $C$ be $A$-algebra and two maps from the initial object $A$ of the category $A$-algebras into $B$ and $C$. Then the $A$-module $B \otimes_A C$ carries an $A$-algebra structure and is the pushout of the diagram $B \leftarrow A \rightarrow C$
	\begin{center}
		\begin{tikzcd}
			& B \arrow[d] \arrow[rd]          &   \\
			A \arrow[ru] \arrow[rd] & B \otimes_A C \arrow[r, dashed] & D \\
			& C \arrow[u] \arrow[ru]          &  
		\end{tikzcd}
	\end{center}
\end{theorem}

\begin{proof}[Construction]
	We will define multiplication on $B \otimes_A C$. Consider the multilinear map
	\begin{align*}
		B \times C \times B \times C &\to B \otimes_A C \\
		(b_1, c_1, b_2, c_2) &\mapsto b_1 b_2 \otimes c_1 c_2
	\end{align*}
	
	The map induces a bilinear map $\mu: (B \otimes C) \times (B \otimes C) \to B \otimes C$
	\begin{center}
		\begin{tikzcd}
			B \times C \times B \times C \arrow[rd] \arrow[d]               &             \\
			(B \otimes C) \otimes (B \otimes C) \arrow[r, dashed]           & B \otimes C \\
			(B \otimes C) \times (B \otimes C) \arrow[u] \arrow[ru, "\mu"'] &            
		\end{tikzcd}
	\end{center}
	
	The multiplicative identity on $B \otimes C$ is $1 \otimes 1$
\end{proof}

\begin{proof}
	\note{TODO - proof the universality}
\end{proof}

\begin{remark}
	Let $B$ be an $A$-algebra (there is a natural map $\phi: A \to B$ defined by $\phi(a) =  a 1_B)$), then
	$$
		B \otimes_A A[x] \xrightarrow{\sim} B[x]
	$$
\end{remark}

\begin{proof}
	The isomorphism as $A$-module can be proven by writing $A[x] = \bigoplus_{n=0}^\infty A$, then $B \otimes A[x] = B \otimes_A \tuple*{\bigoplus_{n=0}^\infty A} = \bigoplus_{n=0}^\infty B \otimes_A A = \bigoplus_{n=0}^\infty B = B[x]$. The proof for $A$-algebra can be done by constructing isomorphisms $f: B \otimes_A A[x] \to B[x]$ and $g: B[x] \to B \otimes_A A[x]$ by
	$$
		f\tuple*{\sum_{i} \tuple*{b_i \otimes \sum_{ij} a_{j} x^j}} = \sum_{i} \sum_{j} a_{ij} b_i x^j
	$$
	$$
		g\tuple*{\sum_{j} b_j x^j} = \sum_{j} b_j \otimes x^j
	$$
	
	(alternative proof using universal property) 
	The image of composition $A \to B \to B[x]$ is identical to the image of the composition $A \to A[x] \to B[x]$ which is the subring $A$ of $B$ in $B[x]$
	\begin{center}
		\begin{tikzcd}
			& B \arrow[d, "\beta"'] \arrow[rd, "f"]       &   \\
			A \arrow[ru] \arrow[rd] & {B[x]} \arrow[r, "h", dashed]               & D \\
			& {A[x]} \arrow[u, "\alpha"] \arrow[ru, "g"'] &  
		\end{tikzcd}
	\end{center}
	
	Let $f: B \to D$ and $g: A[x] \to D$ so that the diagram commutes. We will construct the map $h: B[x] \to D$ so that the diagram commutes. For any $b_n x^n \in B[x]$, define
	$$
		h(b_n x^n) = f(b_n) g(x^n)
	$$
	
	For any $b \in B$, $h \beta(b) = h(b) = f(b)$. For any $a_n x^n \in A[x]$, $h \alpha (a_n x^n) = h(a_n x^n) = f(a_n) g(x^n)$. Note that, $f(a_n) = g(a_n)$, then $h \alpha (a_n x^n) = g(a_n) g(x^n) = g(a_n x^n)$. Hence, the diagram with $h$ commutes
	
	Now, if $h_1: B[x] \to D$ is another map that makes the diagram commutes, then we must have $h_1(b_n) = h_1 \beta (b_n) = f(b_n)$ and $h_1(x^n) = h_1 \alpha(x^n) = g(x^n)$, then
	$$
		h_1(b_n x^n) = h_1(b_n) h_1(x^n) = f(b_n) g(x^n) = h(b_n x^n)
	$$
	
	Hence, $h$ is unique.
\end{proof}

\begin{remark}
	Calculate $\C \otimes_\R \C$
\end{remark}

\begin{proof}
	We have $\C = \R[x] / (x^2 + 1)$, and the exact sequence 
	\begin{center}
		\begin{tikzcd}
			(x^2 + 1) \otimes_\R \C \arrow[r, "i \otimes 1"] & {\R[x] \otimes_\R \C} \arrow[r, two heads] & {\R[x]/(x^2+1) \otimes_\R \C} \arrow[r] & 0
		\end{tikzcd}
	\end{center}
	
	Then 
	\begin{align*}
		\C \otimes_\R \C
		&= \R[x] / (x^2 + 1) \otimes_\R \C \\
		&= (\R[x] \otimes_A \C) / \im (i \otimes 1)
	\end{align*}
	
	We have
	\begin{center}
		\begin{tikzcd}
			(x^2 + 1) \otimes_\R \C \arrow[r, "i \otimes 1"] & {\R[x] \otimes_\R \C} \arrow[r, "\sim"]  & {\C[x]}       \\
			f(x)(x^2+1) \otimes c \arrow[r, maps to]         & f(x)(x^2+1) \otimes c \arrow[r, maps to] & c f(x)(x^2+1)
		\end{tikzcd}
	\end{center}
	
	Hence, $\im (i \otimes 1)$ in $\C[x]$ is the ideal generated by $(x^2 + 1)$, then
	$$
		\C \otimes_\R \C = \C[x] / (x^2 + 1) = \C[x] / (x + i)(x - i)
	$$
	
	By CRT for coprime ideals $(x + i)$ and $(x - i)$
	$$
		\C \otimes_\R \C  = \C[x] / (x + i)(x - i) = \C[x] / (x + i) \times  \C[x] / (x - i) = \C \times \C
	$$
	
	Note that, the map $\C \otimes_\R \C \to \C \times \C$ is defined by $a \otimes b \mapsto (\bar{a} b, ab)$
\end{proof}

\begin{remark}
	For any Galois extension of fields $E / F$
	$$
		E \otimes_F E = E^{\deg(E / F)}
	$$
	
	\note{never studied any field theory - I absolutely have no idea what a Galois extension is}
\end{remark}

\section{TEASER}

\begin{remark}
	$\Tor$ and $\Ext$ functors
\end{remark}

\begin{remark}
	If $L$ is a flat module and the top sequence is exact, then the bottom sequence is also exact
	\begin{center}
		\begin{tikzcd}
			0 \arrow[r] & M \arrow[r]           & N \arrow[r]           & L \arrow[r]           & 0 \\
			0 \arrow[r] & M \otimes P \arrow[r] & N \otimes P \arrow[r] & N \otimes P \arrow[r] & 0
		\end{tikzcd}
	\end{center}
	
	An $A$-module $M$ is flat if and only if for any ideal $I \subseteq A$, the canonical map
	$$
		I \otimes_A M \to IM
	$$
	is an isomorphism
\end{remark}